transformations/Class2Relational/theorems/Relational_resolve.v
@@ -19,10 +19,7 @@ From transformations.Class2Relational
   Require ClassMetamodelProperties RelationalMetamodelProperties.
 
 From transformations.Class2Relational Require Tactics.
-
-
-(* FIXME : move-me *)
-Ltac duplicate H1 H2 := remember H1 as H2 eqn: TMP ; clear TMP.
+From transformations.Class2Relational Require TraceUtils.
 
 
 (** *** Utilities on transformation of elements *)
@@ -53,6 +50,32 @@ Proof.
     reflexivity.
   + auto. 
 Qed.
+Lemma transform_class_fw : 
+  forall (cm : ClassModel) (rm : RelationalModel), 
+  (* transformation *) rm = execute Class2Relational cm ->
+  (* precondition *)  forall id name,
+    In (ClassElement {| class_id:= id ; class_name := name|}) cm.(modelElements) ->
+  (* postcondition *) 
+    In (TableElement {| table_id := id; table_name := name |}) (rm.(modelElements)). 
+Proof.
+  intros cm rm H ; subst.
+  intros i n H.
+  simpl.
+  apply Tactics.allModelElements_allTuples in H.
+  revert H ; generalize (allTuples Class2Relational cm).
+  induction l ; intro H ; [ solve [inversion H] | simpl ].
+  apply List.in_or_app.
+  simpl in H.
+  destruct_or H ; [ left | right ].
+  + subst.
+    clear IHl.
+    compute.
+    left.
+    reflexivity.
+  + auto. 
+
+    (* Remark : exactly the same script as above. *)
+Qed.
 
 (* FIXME : move-me *)
 (* NOT USED *)
@@ -68,6 +91,7 @@ Proof.
   intros cm rm H ; subst.
   intros i n H.
   simpl in H.
+(*  Tactics.in_singleton_allTuples. FIXME : does not work*)
   apply Tactics.allModelElements_allTuples_back with (t:=Class2Relational).
   revert H ; generalize (allTuples Class2Relational cm).
   induction l ; intro H ; [ solve [inversion H] | simpl ].
@@ -88,41 +112,224 @@ Proof.
   + auto.
 Qed.
 
+Lemma transform_class_bw : 
+  forall (cm : ClassModel) (rm : RelationalModel), 
+  (* transformation *) rm = execute Class2Relational cm ->
+  (* precondition *)  forall id name,
+      In (TableElement {| table_id := id; table_name := name |}) (rm.(modelElements)) ->
+  (* postcondition *) 
+    In (ClassElement {| class_id:= id ; class_name := name|}) (cm.(modelElements))
+. 
+Proof.
+  (* Remark : (nearly) same script as above. *)
+  intros cm rm H ; subst.
+  intros i n H.
+  simpl in H.
+  apply Tactics.allModelElements_allTuples_back with (t:=Class2Relational).
+  revert H ; generalize (allTuples Class2Relational cm).
+  induction l ; intro H ; [ solve [inversion H] | simpl ].
+  simpl in H.
+  apply List.in_app_or in H.
+
+  destruct_or H ; [ left | right ].
+  + Tactics.show_singleton.
+    Tactics.show_origin.
+    f_equal.
+    f_equal.
+    destruct c.
+    compute in H.
+    remove_or_false H.
+      injection H ; intros ;subst ; clear H.
+      reflexivity.
+  + auto.
+Qed.
+
+
+
+
+
+(** Concepts under focus in this module *)
+
+Definition all_attributes_are_typed (cm : ClassModel) :=
+  forall (att : Attribute_t),
+      In (AttributeElement att) cm.(modelElements) ->
+      exists (r:Class_t), 
+        In (AttributeTypeLink {| source_attribute := att ; a_type := r |}) cm.(modelLinks) .
+
+Definition all_columns_have_a_reference (rm : RelationalModel) :=
+forall (col: Column_t),
+      In (ColumnElement col) rm.(modelElements) ->
+      exists r', In (ColumnReferenceLink {| cr := col ;  ct := r' |}) rm.(modelLinks).
   
+
+Lemma wf_stable cm rm :
+  rm = execute Class2Relational cm ->
+  all_attributes_are_typed cm ->
+  ClassMetamodelProperties.wf_classmodel_types_exist cm ->
+  ClassMetamodelProperties.wf_classmodel_unique_attribute_types cm ->
+  RelationalMetamodelProperties.wf_all_table_references_exist rm.
+Proof.
+  intros T C_WF1 C_WF2 C_WF3.
+  intros r t R_IN1.
+  subst rm.
+  
+  Tactics.destruct_execute.
+  rename IN_E into C_IN1.
+
+  destruct t.
+  apply transform_class_fw with (cm:=cm) ; [ reflexivity | ]. (* FIXME : don't want to destruct t to be able to apply transform_class_fw. *)
+
+  repeat Tactics.destruct_any.
+  
+  clear IN0.
+  
+  (* on a besoin de savoir quelle règle a été appliquée pour progresser dans le calcul *)
+  Tactics.destruct_In_two ; simpl in * ; 
+  remove_or_false_auto ; subst ; simpl in * ;
+  Tactics.deduce_element_kind_from_guard ; simpl in * ;
+  [ | ].
+  { (* first rule : impossible *)
+    exfalso.
+
+    (* Set Printing All.*)
+
+    eapply Tactics.allModelElements_allTuples_back with (t:=Class2Relational) in C_IN1 ;
+    (* FIXME : the tactics does not work*)
+      simpl in *.
+    repeat Tactics.destruct_any.
+    unfold Parser.parseOutputPatternElement in IN2 ; simpl in *. 
+    unfold applyElementOnPattern in IN2 ; simpl in IN2.
+        
+    rewrite app_nil_r in IN2.
+    Tactics.destruct_in_optionListToList.
+    
+    unfold Parser.parseOutputPatternLink in M ; simpl in M.
+    unfold ConcreteExpressions.makeLink in M ; simpl in M.
+    unfold ConcreteExpressions.wrapLink in M ; simpl in M.
+     
+    Tactics.monadInv M.
+    unfold maybeBuildTableColumns in M.
+    
+    Tactics.monadInv M.
+    apply in_singleton in IN2 ; discriminate IN2.
+  }
+  {
+    (* second rule *)
+
+    (* Set Printing All.*)
+    eapply Tactics.allModelElements_allTuples_back with (t:=Class2Relational) in C_IN1 ;
+    (* FIXME : the tactics does not work*)
+      simpl in *.
+    repeat Tactics.destruct_any.
+    unfold Parser.parseOutputPatternElement in IN2 ; simpl in *. 
+    unfold applyElementOnPattern in IN2 ; simpl in IN2.
+        
+    rewrite app_nil_r in IN2.
+    Tactics.destruct_in_optionListToList.
+    
+    unfold Parser.parseOutputPatternLink in M ; simpl in M.
+    unfold ConcreteExpressions.makeLink in M ; simpl in M.
+    unfold ConcreteExpressions.wrapLink in M ; simpl in M ;
+      Tactics.monadInv M.
+
+    apply in_singleton in IN2 ; Tactics.inj IN2.
+    
+    unfold maybeBuildColumnReference in M ; 
+      Tactics.monadInv M.
+
+    unfold ModelingSemantics.maybeResolve in M ;
+      simpl in M.
+
+    unfold ModelingSemantics.denoteOutput in M ; 
+      Tactics.monadInv M.
+
+    Ltac toEDataT H :=
+      match type of H with
+        toEData Table_K ?E = Some _ => destruct E ; [ | discriminate H] 
+      end.
+
+    toEDataT M.
+    destruct t ; unfold toEData in M ; simpl in M ; Tactics.inj M.
+
+    destruct a (* FIXME *). simpl in D ; subst derived.
+
+    unfold maybeResolve in E ; 
+      Tactics.monadInv E.
+  
+    unfold maybeSingleton in E0.
+    unfold option_map in E0 ;
+      Tactics.monadInv E0.
+
+    unfold getAttributeTypeElement in E0.
+    Tactics.monadInv E0.
+
+    unfold singleton in E ; simpl in E.
+    
+    Tactics.duplicate C_IN1 C_IN2.
+    apply C_WF1 in C_IN2 ; destruct C_IN2 as (t & C_IN2).
+    rewrite ClassMetamodelProperties.getAttributeType_In_left_3 with (t:=t) in E0 ;
+      [ | exact C_WF3 | exact C_IN2]. 
+    Tactics.inj E0.    
+ 
+    unfold resolve in E.
+    unfold resolveIter in E ;
+      Tactics.monadInv E.
+
+
+    destruct t ; simpl in * ; subst.  
+
+    apply find_some in E ; simpl in *.
+    destruct E as (T_IN1 & T_IN2).
+    
+    specialize (TraceUtils.trace_wf cm) ; intro T_WF.
+    unfold TraceUtils.wf in T_WF.
+    eapply List.Forall_forall in T_WF ; [ | exact T_IN1 ].
+    inversion T_WF ; subst.
+    destruct c ; subst ; simpl in *.
+    
+    eapply TraceUtils.in_trace_in_models in T_IN1 ; 
+      destruct T_IN1 as (IN1 & IN2). 
+    destruct c0 ; assumption.
+  }
+Qed.
+
 (** *** Result *)
 
-From transformations.Class2Relational Require TraceUtils.
 
-Theorem Relational_Column_Reference_definedness:
+
+Theorem Relational_Column_Reference_definedness_aux:
 forall (cm : ClassModel) (rm : RelationalModel), 
+
+  (* well-formed *) ClassMetamodelProperties.wf_classmodel_types_exist cm ->
 
   (* transformation *) rm = execute Class2Relational cm ->
 
-  (* precondition *)  (forall (att : Attribute_t),
-      In (AttributeElement att) cm.(modelElements) ->
-      exists (r:Class_t), 
-        getAttributeType att cm = Some r 
-        /\ In (ClassElement r) cm.(modelElements) (* well-formed *) ) ->  
+  (* precondition *) all_attributes_are_typed cm  ->  
 
-    (* postcondition *)  forall (col: Column_t),
-      In (ColumnElement col) rm.(modelElements) ->
-      exists r', getColumnReference col rm =Some r'. 
+    (* postcondition *) all_columns_have_a_reference rm . 
 
 Proof. 
-  intros cm rm E PRE.  intros col I1.
+  intros cm rm  WF2 E PRE.  intros col IN1. 
   subst rm.
-  Tactics.destruct_execute.
-  Tactics.show_singleton.
-  Tactics.show_origin.
+  repeat Tactics.destruct_execute.
+  repeat Tactics.show_singleton.
+  repeat Tactics.show_origin.
   repeat Tactics.destruct_any.
+
+  (* we have lost IN1 : In (ColumnElement col)
+          (modelElements (execute Class2Relational cm)) *)
 
   clear IN_I. 
   
   apply Tactics.allModelElements_allTuples_back in IN_E.
   
-  specialize (PRE _ IN_E).
-  destruct PRE as (t & (PRE1 & PRE2)).
- 
+  Tactics.duplicate PRE H.
+
+  specialize (H _ IN_E).
+  destruct H as (c & G1).
+  Tactics.duplicate G1 IN_C ; apply WF2 in IN_C.  
+  
+  Tactics.duplicate G1 IN2. 
   unfold getColumnReference.
 
   unfold execute.  simpl. 
@@ -130,7 +337,7 @@ Proof.
   set (z:=r).
 
   Tactics.destruct_In_two ; [ exfalso | ] ; 
-   simpl in IN_OP ; remove_or_false IN_OP ; subst ope ; [ discriminate I1 | Tactics.inj I1]. 
+   simpl in IN_OP ; remove_or_false IN_OP ; subst ope ; [ discriminate IN1 | Tactics.inj IN1]. 
   
   clear n. 
   simpl in M.
@@ -140,15 +347,143 @@ Proof.
   destruct a0 ; simpl in *. (* derived a0 = false *)
   subst derived ; simpl in *. 
 
-  duplicate PRE1 G1.
-  apply ClassMetamodelProperties.get_in in PRE1.
+  Tactics.duplicate G1 G2. (* à quoi sert de garder PRE1 ? *)
 
-  specialize (TraceUtils.in_maybeResolve_trace_2 t cm PRE2 ) ; intros (R & I).
+
+  specialize (TraceUtils.in_maybeResolve_trace_2 c cm IN_C ) ; 
+    intros (R & I).
+
+
+  apply ClassMetamodelProperties.getAttributeType_In_left_2 in G1 ;
+    destruct G1 as [r G1].
+
+  exists{| table_id := r.(class_id); table_name := r.(class_name) |}.
+
+  apply in_flat_map.
+  exists ([AttributeElement {|
+               attr_id := attr_id;
+               derived := false;
+               attr_name := attr_name
+             |}]).
+  split.
+  { apply Tactics.allModelElements_allTuples. exact IN_E. }
+  {
+    
+    unfold applyPattern.
+    apply in_flat_map.
+    exists z.
+    
+    split.
+    { subst z. simpl. auto. }
+    { 
+      apply tr_applyRuleOnPattern_in ; simpl.
+      exists 0.
+      split ; [ solve [auto] | ].
+      apply tr_applyIterationOnPattern_in.
+      eexists  ; split ; [ solve [subst z ; simpl ; auto] | ].
+      erewrite tr_applyElementOnPattern_leaf ; simpl.
+      2:{ compute. reflexivity. }
+
+      rewrite <- app_nil_end. 
+      simpl.
+      
+      unfold Parser.parseOutputPatternLink ; simpl.
+      unfold ConcreteExpressions.makeLink ; simpl.
+      unfold ConcreteExpressions.wrapLink ; simpl.
+      unfold getAttributeTypeElement.
+     
+      
+
+      rewrite G1.
+
+
+
+      unfold ModelingSemantics.maybeResolve.
+
+      apply ClassMetamodelProperties.getAttributeType_classex in G1 ; [ | exact WF2].
+
+      apply TraceUtils.in_maybeResolve_trace_2 in G1.
+      destruct G1 as (G11 & G12).
+      
+      unfold maybeSingleton.
+      unfold option_map.
+      unfold singleton.
+      rewrite G11.
+      simpl.
+      left.
+      reflexivity.
+    }
+  }
+Qed.
+
+
+Theorem Relational_Column_Reference_definedness:
+forall (cm : ClassModel) (rm : RelationalModel), 
+
+(* well-formed *) ClassMetamodelProperties.wf_classmodel_types_exist cm ->
+
+  (* transformation *) rm = execute Class2Relational cm ->
+
+  (* precondition *)  (forall (att : Attribute_t),
+      In (AttributeElement att) cm.(modelElements) ->
+      exists (r:Class_t), 
+        getAttributeType att cm = Some r ) ->  
+
+    (* postcondition *)  forall (col: Column_t),
+      In (ColumnElement col) rm.(modelElements) ->
+      exists r', getColumnReference col rm =Some r'. 
+
+Proof. 
+  intros cm rm WF E PRE.  intros col IN1.
+  subst rm.
+
+  repeat Tactics.destruct_execute.
+  repeat Tactics.show_singleton.
+  repeat Tactics.show_origin.
+  repeat Tactics.destruct_any.
+
+  (* we have lost IN1 : In (ColumnElement col)
+          (modelElements (execute Class2Relational cm)) *)
+
+  clear IN_I. 
+  
+  apply Tactics.allModelElements_allTuples_back in IN_E.
+  
+  Tactics.duplicate PRE H.
+
+  specialize (H _ IN_E).
+  destruct H as (c & G1). 
+  Tactics.duplicate G1 IN_C.
+  apply ClassMetamodelProperties.getAttributeType_In_right in IN_C.
+  eapply WF in IN_C.
+  Tactics.duplicate G1 IN2. (* test *)
+  apply ClassMetamodelProperties.getAttributeType_In_right in IN2.
+  unfold getColumnReference.
+
+  unfold execute.  simpl. 
+
+  set (z:=r).
+
+  Tactics.destruct_In_two ; [ exfalso | ] ; 
+   simpl in IN_OP ; remove_or_false IN_OP ; subst ope ; [ discriminate IN1 | Tactics.inj IN1]. 
+  
+  clear n. 
+  simpl in M.
+  
+  Tactics.deduce_element_kind_from_guard. (* M *)
+ 
+  destruct a0 ; simpl in *. (* derived a0 = false *)
+  subst derived ; simpl in *. 
+
+  Tactics.duplicate G1 G2. (* à quoi sert de garder PRE1 ? *)
+  apply ClassMetamodelProperties.getAttributeTypeOnLinks_in in G1.
+
+  specialize (TraceUtils.in_maybeResolve_trace_2 c cm IN_C ) ; intros (R & I).
 
 
   eapply RelationalMetamodelProperties.in_get_2_right 
-    with (x:= {| table_id :=t.(class_id) ;  
-                table_name := t.(class_name) |}) . 
+    with (x:= {| table_id := c.(class_id) ;  
+                table_name := c.(class_name) |}) . 
 
     apply in_flat_map.
     exists ([AttributeElement {|
@@ -182,7 +517,7 @@ Proof.
       unfold ConcreteExpressions.makeLink ; simpl.
       unfold ConcreteExpressions.wrapLink ; simpl.
       unfold getAttributeTypeElement.
-      rewrite G1. simpl.
+      rewrite G2. simpl.
 
       unfold ModelingSemantics.maybeResolve.
       unfold singleton.
@@ -194,3 +529,97 @@ Proof.
 Qed.
      
 
+
+
+Theorem Relational_Column_Reference_definedness_altproof:
+  forall (cm : ClassModel) (rm : RelationalModel), 
+    
+    (* well-formed *) ClassMetamodelProperties.wf_classmodel_types_exist cm ->
+    
+    (* transformation *) rm = execute Class2Relational cm ->
+    
+    (* precondition *)  (forall (att : Attribute_t),
+        In (AttributeElement att) cm.(modelElements) ->
+        exists (r:Class_t), 
+          getAttributeType att cm = Some r ) ->  
+    
+      (* postcondition *)  forall (col: Column_t),
+        In (ColumnElement col) rm.(modelElements) ->
+        exists r', getColumnReference col rm =Some r'. 
+
+Proof. 
+  intros cm rm WF E PRE.  intros col IN1.
+  cut (all_columns_have_a_reference rm).
+  {
+    intro WT.
+    unfold all_columns_have_a_reference in WT.
+    apply WT in IN1.
+    destruct IN1 as (r & IN2).
+    apply RelationalMetamodelProperties.in_get_2_right_2.
+    eauto.
+  }
+  {
+    apply Relational_Column_Reference_definedness_aux with (cm:=cm) ;
+    [ exact WF | exact E | ].
+    unfold all_attributes_are_typed.
+    intros att IN2.
+    apply PRE in IN2.
+    destruct IN2 as (r & G).
+    apply ClassMetamodelProperties.getAttributeType_In_right in G.
+    eauto.
+  }
+Qed.
+
+
+Corollary Relational_Column_Reference_definedness_2:
+  forall (cm : ClassModel) (rm : RelationalModel), 
+    
+    (* well-formed (1/2) *) 
+    ClassMetamodelProperties.wf_classmodel_types_exist cm ->
+    
+    (* well-formed (2/2) *) 
+    ClassMetamodelProperties.wf_classmodel_unique_attribute_types cm ->
+    
+    (* transformation *) 
+    rm = execute Class2Relational cm ->
+    
+    (* precondition *)  
+    (forall (att : Attribute_t),
+        In (AttributeElement att) cm.(modelElements) ->
+        exists (r:Class_t), 
+          getAttributeType att cm = Some r ) ->  
+    
+    (* postcondition *)  
+    forall (col: Column_t),
+        In (ColumnElement col) rm.(modelElements) ->
+        exists r', (getColumnReference col rm = Some r' 
+                    /\ In (TableElement r') rm.(modelElements)). 
+
+Proof. 
+  intros cm rm WF1 WF2 T WF3 col IN .
+  cut (exists r' : Table_t,
+          getColumnReference col rm = return r').
+  {
+    intros (r & G).
+    exists r.
+    split ; [ exact G | ].
+    eapply wf_stable ; [ exact T |  | exact WF1  | exact WF2 | ].
+    {
+      (* comes from WF3 *)
+      unfold all_attributes_are_typed.  
+      intros att IN2.
+      apply WF3 in IN2.
+      destruct IN2 as (r2 & G2).
+      apply ClassMetamodelProperties.getAttributeType_In_right in G2.
+      eauto.
+    }
+    {
+      (* comes from G *)
+      apply RelationalMetamodelProperties.in_get_2_left.
+      exact G.
+    }
+  }
+  {
+    eapply Relational_Column_Reference_definedness ; eassumption.
+  }
+Qed.
